q2

A1/q2.js
@@ -1,10 +1,36 @@
-function min(a, left, right) {
-    if (a[left] > a[right]) {
-        return a[right];
+
+function findMin(a, left, right) {
+    if (left < right)  {
+        if (a[left] < a[right]) { 
+            return findMin(a, left, right - 1);
+        } else {
+            return findMin(a, left + 1, right);
+        }
     } else {
-        return a[left];
+        return left;
     }
 }
 
-var a = [1,3,6,8,2,9,10,4,0];
-console.log(a[1,2]);
+function stoogeSort(a, left, right) {
+    console.log("Find min index = " + findMin(a, left, right) );
+    console.log("Array = " + a);
+    console.log("Left = " + left + " Right = " + right + " Ele = " + a[findMin(a, left, right)]);
+    if (a[left] > a[right]) {
+        var tmp = a[left];
+        a[left] = a[right];
+        a[right] = tmp;
+    }
+    if (left + 1 >= right) {
+        return;
+    }
+    var k = Math.floor((right - left + 1) / 3);
+    stoogeSort(a, left, right - k); // First two-thirds
+    stoogeSort(a, left + k, right); // Last two-thirds
+    stoogeSort(a, left, right - k); // First two-thirds again
+}
+
+
+var a = [1,2,7,2,8,0,10];
+var a = [2, 4, 5, 3, 1];
+stoogeSort(a, 0, a.length - 1);
+console.log(a);
